

### 3. Solution of Linear Equations using Matrices

#### A. Activities

Carry out the following activities to solve the equations.

1.  $x - y + z = 1$ ,  $2x - y = 1$ ,  $3x + 3y - 4z = 2$

**Solution :** The given equation can be written as

$$\begin{bmatrix} 1 & -1 & 1 \\ 2 & -1 & 0 \\ 3 & 3 & -4 \end{bmatrix} \begin{bmatrix} x \\ y \\ z \end{bmatrix} = \begin{bmatrix} 1 \\ 1 \\ 2 \end{bmatrix}$$

By  $R_2 - 2R_1$  and  $R_3 - 3R_1$

$$\begin{bmatrix} 1 & -1 & 1 \\ 0 & 1 & -2 \\ 0 & 0 & 5 \end{bmatrix} X = \begin{bmatrix} 1 \\ -1 \\ -1 \end{bmatrix} \text{ where } X = \begin{bmatrix} x \\ y \\ z \end{bmatrix}$$

By  $R_3 - 6R_2$

$$\begin{bmatrix} 1 & -1 & 1 \\ 0 & 1 & -2 \\ 0 & 0 & 5 \end{bmatrix} \begin{bmatrix} x \\ y \\ z \end{bmatrix} = \begin{bmatrix} 1 \\ -1 \\ 5 \end{bmatrix}$$

$$\begin{bmatrix} x - y + z \\ y - 2z \\ 5z \end{bmatrix} = \begin{bmatrix} 1 \\ -1 \\ 5 \end{bmatrix}$$

By equality of matrices

$$\boxed{x} - \boxed{y} + \boxed{z} = 1 \quad \dots\dots\dots (1)$$

$$\boxed{y} - 2\boxed{z} = \boxed{-1} \quad \dots\dots\dots (2)$$

$$\boxed{5}z = \boxed{5} \quad \dots\dots\dots (3)$$

From (3)  $z = \boxed{1}$ , from (2), we get  $y = \boxed{1}$

Substituting  $y = \boxed{1}$ ,  $z = \boxed{1}$  in (1), we get  $x = \boxed{1}$

2. The cost of 4 pencils, 3 pens and 2 erasers is ₹ 60. The cost of 2 pencils, 4 pens and 6 erasers is ₹ 90. The cost of 6 pencils, 2 pens and 3 erasers is ₹ 70. Find the cost of each item, using the following activity.

**Solution :** Let the cost of 1 pencil, 1 pen and 1 eraser be ₹  $x$ , ₹  $y$ , ₹  $z$  respectively.

Then  $4x + \boxed{3}y + \boxed{2}z = \boxed{60}$

$$x + \boxed{2}y + \boxed{3}z = \boxed{45}$$

$$6x + \boxed{2}y + \boxed{3}z = 70$$

These equation can be written as

$$\begin{bmatrix} 4 & 3 & 2 \\ 1 & 2 & 3 \\ 6 & 2 & 3 \end{bmatrix} X = \begin{bmatrix} 60 \\ 45 \\ 70 \end{bmatrix} \text{ where } X = \begin{bmatrix} x \\ y \\ z \end{bmatrix}$$

$$\text{By } R_1 \leftrightarrow R_2 \begin{bmatrix} 1 & 2 & 3 \\ 4 & 3 & 2 \\ 6 & 2 & 3 \end{bmatrix} X = \begin{bmatrix} 45 \\ 60 \\ 70 \end{bmatrix}$$

By  $R_2 - 4R_1$  and  $R_3 - 6R_1$

$$\begin{bmatrix} 1 & 2 & 3 \\ 0 & -5 & -10 \\ 0 & -10 & -15 \end{bmatrix} X = \begin{bmatrix} 45 \\ -120 \\ -200 \end{bmatrix}, \text{ By } R_3 - 2R_2$$

$$\begin{bmatrix} 1 & 2 & 3 \\ 0 & -5 & -10 \\ 0 & 0 & 5 \end{bmatrix} \begin{bmatrix} x \\ y \\ z \end{bmatrix} = \begin{bmatrix} 45 \\ -120 \\ 40 \end{bmatrix}$$

$$\therefore x + 2y + 3z = 45 \dots\dots\dots (1) \quad -5y - 10z = -120 \dots\dots\dots (2)$$

$$0x + 0y + 5z = 40 \dots\dots\dots (3) \text{ we get } z = 8$$

$$\text{From (2) } y = 8, \text{ from (1) } x = 5$$

3. Express the following equation in matrix form and solve them using method of inversion by completing the following activity.

$$x + 2y + 3z = 6, \quad x + y + 5z = 7, \quad 2x + 4y + 7z = 13$$

$$\text{Solution : Let } A = \begin{bmatrix} 1 & 2 & 3 \\ 1 & 1 & 5 \\ 2 & 4 & 7 \end{bmatrix}, \quad |A| = -1 \neq 0 \quad A^{-1} \text{ exists.}$$

$$A_{11} = (-1)^{1+1} M_{11} = (1) \begin{vmatrix} 1 & 5 \\ 4 & 7 \end{vmatrix} = 7 - 20 = -13$$

$$A_{12} = (-1)^{1+2} M_{12} = (-1) \begin{vmatrix} 1 & 5 \\ 2 & 7 \end{vmatrix} = 3$$

$$A_{13} = (-1)^{1+3} M_{13} = (1) \begin{vmatrix} 1 & 1 \\ 2 & 4 \end{vmatrix} = 2$$

$$A_{21} = (-1)^{2+1} M_{21} = (-1) \begin{vmatrix} 2 & 3 \\ 4 & 7 \end{vmatrix} = -2$$

$$A_{22} = (-1)^{2+2} M_{22} = (1) \begin{vmatrix} 1 & 3 \\ 2 & 7 \end{vmatrix} = 1$$

$$A_{23} = (-1)^{2+3} M_{23} = (-1) \begin{vmatrix} 1 & 2 \\ 2 & 4 \end{vmatrix} = 0$$

$$A_{31} = (-1)^{3+1} M_{31} = (-1) \begin{vmatrix} 2 & 3 \\ 1 & 5 \end{vmatrix} = \dots 7 \dots$$

$$A_{32} = (-1)^{3+2} M_{32} = (-1) \begin{vmatrix} 1 & 3 \\ 1 & 5 \end{vmatrix} = \dots -2 \dots$$

$$A_{33} = (-1)^{3+3} M_{33} = (1) \begin{vmatrix} 1 & 2 \\ 1 & 1 \end{vmatrix} = \boxed{1} - \boxed{2} = \boxed{-1}$$

$$\text{adj } A = \begin{bmatrix} \boxed{-13} & -2 & \boxed{7} \\ 3 & \boxed{1} & -2 \\ \boxed{2} & 0 & \boxed{-1} \end{bmatrix}$$

$$A^{-1} = \begin{bmatrix} \boxed{13} & 2 & \boxed{-7} \\ -3 & -1 & 2 \\ \boxed{-2} & 0 & \boxed{1} \end{bmatrix}$$

Now  $AX = B$

Premultiplying by  $A^{-1}$  we get,

$$A^{-1}AX = A^{-1}B$$

$$IX = A^{-1}B$$

$$X = \begin{bmatrix} \boxed{13} & 2 & \boxed{-7} \\ -3 & \boxed{-1} & 2 \\ \boxed{-2} & 0 & \boxed{1} \end{bmatrix} \begin{bmatrix} 6 \\ 7 \\ 13 \end{bmatrix}$$

$$X = \begin{bmatrix} \boxed{1} \\ \boxed{1} \\ \boxed{1} \end{bmatrix}$$

$$\therefore x = \boxed{1}, y = \boxed{1}, z = \boxed{1}$$

B. Solve the Following

Q.1 The cost of 4 kg potato, 3 kg wheat, and 2 kg rice is Rs. 60. The cost of 1 kg potato, 2 kg wheat, and 3 kg rice is Rs. 45. The cost of 6 kg potato, 2 kg wheat, and 3 kg rice is Rs. 70. Find the per kg cost of each item by matrix method.

Let ₹  $x$  be the cost of 1 kg potato.

₹  $y$  be the cost of 1 kg wheat.

₹  $z$  be the cost of 1 kg rice.

$$\therefore \text{From the 1st condition, } 4x + 3y + 2z = 60 \quad \text{--- (1)}$$

$$\text{From the 2nd condition, } x + 2y + 3z = 45 \quad \text{--- (2)}$$

$$\& \text{ from the 3rd condition, } 6x + 2y + 3z = 70 \quad \text{--- (3)}$$

$\therefore$  The matrix form of these eq<sup>ns</sup> is



$$\begin{bmatrix} 4 & 3 & 2 \\ 1 & 2 & 3 \\ 6 & 2 & 3 \end{bmatrix} \begin{bmatrix} x \\ y \\ z \end{bmatrix} = \begin{bmatrix} 60 \\ 45 \\ 70 \end{bmatrix}$$

Applying  $R_1 \leftrightarrow R_2$ ,  $\begin{bmatrix} 1 & 2 & 3 \\ 4 & 3 & 2 \\ 6 & 2 & 3 \end{bmatrix} \begin{bmatrix} x \\ y \\ z \end{bmatrix} = \begin{bmatrix} 45 \\ 60 \\ 70 \end{bmatrix}$

By  $R_2 \rightarrow R_2 - 4R_1$ ,  $\begin{bmatrix} 1 & 2 & 3 \\ 0 & -5 & -10 \\ 6 & 2 & 3 \end{bmatrix} \begin{bmatrix} x \\ y \\ z \end{bmatrix} = \begin{bmatrix} 45 \\ -120 \\ 70 \end{bmatrix}$

By  $R_3 \rightarrow R_3 - 6R_1$ ,  $\begin{bmatrix} 1 & 2 & 3 \\ 0 & -5 & -10 \\ 0 & -10 & -15 \end{bmatrix} \begin{bmatrix} x \\ y \\ z \end{bmatrix} = \begin{bmatrix} 45 \\ -120 \\ -200 \end{bmatrix}$

By  $R_2 \rightarrow (-1/5)R_2$  and  $R_3 \rightarrow (-1/5)R_3$

$$\begin{bmatrix} 1 & 2 & 3 \\ 0 & 1 & 2 \\ 0 & 2 & 3 \end{bmatrix} \begin{bmatrix} x \\ y \\ z \end{bmatrix} = \begin{bmatrix} 45 \\ 24 \\ 40 \end{bmatrix}$$

By  $R_3 \rightarrow R_3 - 2R_2$ ,  $\begin{bmatrix} 1 & 2 & 3 \\ 0 & 1 & 2 \\ 0 & 0 & -1 \end{bmatrix} \begin{bmatrix} x \\ y \\ z \end{bmatrix} = \begin{bmatrix} 45 \\ 24 \\ -8 \end{bmatrix}$

$$\therefore x + 2y + 3z = 45 \quad (4), \quad y + 2z = 24 \quad (5)$$

and  $-z = -8 \Rightarrow \boxed{z = 8}$

$\therefore$  Substituting  $z = 8$  in eq<sup>n</sup> (5),  $y + 2(8) = 24 \Rightarrow \boxed{y = 8}$

$\therefore$  from (4),  $x + 2(8) + 3(8) = 45$

$$\Rightarrow x = 45 - 16 - 24 \Rightarrow \boxed{x = 5}$$

Hence, the cost of 1 kg potato = ₹ 5, cost of 1 kg wheat = ₹ 8 and cost of 1 kg rice = ₹ 8.

Q.2 Solve the following equations by the method of inversion.

(i)  $x + y = 1, y + z = \frac{5}{3}, z + x = \frac{4}{3}$ .

[Find  $A^{-1}$  using row transformations.]

The give equations can be written in the matrix form as,

$$AX=B$$

Pre-multiplying by  $A^{-1}$ ,

$$A^{-1}AX = A^{-1}B$$

$$\Rightarrow X = A^{-1}B \quad \text{--- (1)}$$

Consider  $AA^{-1} = I$

$$\begin{bmatrix} 1 & 1 & 0 \\ 0 & 3 & 3 \\ 3 & 0 & 3 \end{bmatrix} A^{-1} = \begin{bmatrix} 1 & 0 & 0 \\ 0 & 1 & 0 \\ 0 & 0 & 1 \end{bmatrix}$$

By  $R_3 \rightarrow R_3 - 3R_1$  and  $R_2 \rightarrow (1/3)R_2$

$$\begin{bmatrix} 1 & 1 & 0 \\ 0 & 1 & 1 \\ 0 & -3 & 3 \end{bmatrix} A^{-1} = \begin{bmatrix} 1 & 0 & 0 \\ 0 & 1/3 & 0 \\ -3 & 0 & 1 \end{bmatrix}$$

By  $R_3 \rightarrow R_3 + 3R_2$

$$\begin{bmatrix} 1 & 1 & 0 \\ 0 & 1 & 1 \\ 0 & 0 & 6 \end{bmatrix} A^{-1} = \begin{bmatrix} 1 & 0 & 0 \\ 0 & 1/3 & 0 \\ -3 & 1 & 1 \end{bmatrix}$$

By  $R_3 \rightarrow (1/6)R_3$ ,  $R_2 \rightarrow R_2 - R_3$

$$\begin{bmatrix} 1 & 1 & 0 \\ 0 & 1 & 1 \\ 0 & 0 & 1 \end{bmatrix} A^{-1} = \begin{bmatrix} 1 & 0 & 0 \\ 0 & 1/3 & 0 \\ -1/2 & 1/6 & 1/6 \end{bmatrix}$$

By  $R_2 \rightarrow R_2 - R_3$ ,  $R_1 \rightarrow R_1 - R_2$

$$\begin{bmatrix} 1 & 0 & 0 \\ 0 & 1 & 0 \\ 0 & 0 & 1 \end{bmatrix} A^{-1} = \begin{bmatrix} 1/2 & -1/6 & 1/6 \\ 1/2 & 1/6 & -1/6 \\ -1/2 & 1/6 & 1/6 \end{bmatrix}$$

$$\therefore A^{-1} = \begin{bmatrix} 1/2 & -1/6 & 1/6 \\ 1/2 & 1/6 & -1/6 \\ -1/2 & 1/6 & 1/6 \end{bmatrix}$$

$\therefore$  from eq<sup>n</sup> (1)

$$X = \begin{bmatrix} 1/2 & -1/6 & 1/6 \\ 1/2 & 1/6 & -1/6 \\ -1/2 & 1/6 & 1/6 \end{bmatrix} \begin{bmatrix} 1 \\ 5 \\ 4 \end{bmatrix}$$

$$= \begin{bmatrix} 1/2 - 5/6 + 4/6 \\ 1/2 + 5/6 - 4/6 \\ -1/2 + 5/6 + 4/6 \end{bmatrix} = \begin{bmatrix} 1/3 \\ 2/3 \\ 1 \end{bmatrix}$$

$$\therefore x = 1/3, y = 2/3, z = 1$$

(ii)  $x + y + z = 6$ ,  $3x - y + 3z = 10$ ,  $5x + 5y - 4z = 3$ .

[Find  $A^{-1}$  using adjoint method.]

The matrix form of above eq<sup>ns</sup> is  $AX=B$  --- (1)

$$\begin{bmatrix} 1 & 1 & 1 \\ 3 & -1 & 3 \\ 5 & 5 & -4 \end{bmatrix} \begin{bmatrix} x \\ y \\ z \end{bmatrix} = \begin{bmatrix} 6 \\ 10 \\ 3 \end{bmatrix}$$



Now to find  $A^{-1}$  using adjoint method,

$$|A| = 1(4-15) - 1(-12-15) + 1(15+5) = 36 \neq 0$$

$\therefore A^{-1}$  exists.

$$A_{11} = (-1)^{1+1} M_{11} = \begin{vmatrix} -1 & 3 \\ 5 & -4 \end{vmatrix} = 4 - 15 = -11$$

$$A_{12} = (-1)^{1+2} M_{12} = (-1) \begin{vmatrix} 3 & 3 \\ 5 & -4 \end{vmatrix} = -(-12 - 15) = 27$$

$$A_{13} = (-1)^{1+3} M_{13} = \begin{vmatrix} 3 & -1 \\ 5 & 5 \end{vmatrix} = 15 - (-5) = 20$$

$$A_{21} = (-1)^{2+1} M_{21} = (-1) \begin{vmatrix} 1 & 1 \\ 5 & -4 \end{vmatrix} = -(-4 - 5) = 9$$

$$A_{22} = (-1)^{2+2} M_{22} = \begin{vmatrix} 1 & 1 \\ 5 & -4 \end{vmatrix} = -9$$

$$A_{23} = (-1)^{2+3} M_{23} = (-1) \begin{vmatrix} 1 & 1 \\ 5 & 5 \end{vmatrix} = -(5 - 5) = 0$$

$$A_{31} = (-1)^{3+1} M_{31} = \begin{vmatrix} 1 & 1 \\ -1 & 3 \end{vmatrix} = 3 - (-1) = 4$$

$$A_{32} = (-1)^{3+2} M_{32} = (-1) \begin{vmatrix} 1 & 1 \\ 3 & 3 \end{vmatrix} = -(3 - 3) = 0$$

$$A_{33} = (-1)^{3+3} M_{33} = \begin{vmatrix} 1 & 1 \\ 3 & -1 \end{vmatrix} = -1 - 3 = -4$$

$$\therefore \text{Cofactor matrix} = \begin{bmatrix} -11 & 27 & 20 \\ 9 & -9 & 0 \\ 4 & 0 & -4 \end{bmatrix}.$$

$$\therefore \text{Now, } \text{adj}(A) = \begin{bmatrix} -11 & 9 & 4 \\ 27 & -9 & 0 \\ 20 & 0 & -4 \end{bmatrix}$$

$$\therefore A^{-1} = \frac{1}{|A|} \text{adj}(A) = \frac{1}{36} \begin{bmatrix} -11 & 9 & 4 \\ 27 & -9 & 0 \\ 20 & 0 & -4 \end{bmatrix}$$

Premultiplying eqn ① by  $A^{-1}$ , we get,  $X = A^{-1}B$

$$\therefore X = \frac{1}{36} \begin{bmatrix} -11 & 9 & 4 \\ 27 & -9 & 0 \\ 20 & 0 & -4 \end{bmatrix} \begin{bmatrix} 6 \\ 10 \\ 3 \end{bmatrix} = \frac{1}{36} \begin{bmatrix} -66 + 90 + 12 \\ 162 - 90 + 0 \\ 120 - 0 - 12 \end{bmatrix} = \frac{1}{36} \begin{bmatrix} 36 \\ 72 \\ 108 \end{bmatrix} = \begin{bmatrix} 1 \\ 2 \\ 3 \end{bmatrix}$$

$$\therefore x=1, y=2 \text{ \& } z=3$$

Q.3 Solve the following equations by the method of reduction.  
 $x + 3y + 2z = 6$ ,  $3x - 2y + 5z = 5$ ,  $2x - 3y + 6z = 7$ .

The matrix form of above given equation is

$$\begin{bmatrix} 1 & 3 & 2 \\ 3 & -2 & 5 \\ 2 & -3 & 6 \end{bmatrix} \begin{bmatrix} x \\ y \\ z \end{bmatrix} = \begin{bmatrix} 6 \\ 5 \\ 7 \end{bmatrix}$$

By  $R_2 \rightarrow R_2 - 3R_1$ ,

$$\begin{bmatrix} 1 & 3 & 2 \\ 0 & -11 & -1 \\ 2 & -3 & 6 \end{bmatrix} \begin{bmatrix} x \\ y \\ z \end{bmatrix} = \begin{bmatrix} 6 \\ -13 \\ 7 \end{bmatrix}$$

By  $R_3 \rightarrow R_3 - 2R_1$

$$\begin{bmatrix} 1 & 3 & 2 \\ 0 & -11 & -1 \\ 0 & -9 & 2 \end{bmatrix} \begin{bmatrix} x \\ y \\ z \end{bmatrix} = \begin{bmatrix} 6 \\ -13 \\ -5 \end{bmatrix}$$

By  $R_3 \rightarrow R_3 + 2R_2$ ,

$$\begin{bmatrix} 1 & 3 & 2 \\ 0 & -11 & -1 \\ 0 & -31 & 0 \end{bmatrix} \begin{bmatrix} x \\ y \\ z \end{bmatrix} = \begin{bmatrix} 6 \\ -13 \\ -31 \end{bmatrix}$$

$$\therefore x + 3y + 2z = 6 \quad \text{--- (1)}$$

$$-11y - z = -13 \quad \text{--- (2)}$$

$$-31y = -31$$

$$\Rightarrow \boxed{y = 1}$$

$$\text{from (2), } -11(1) - z = -13$$

$$\therefore z = -11 + 13 = 2$$

$$\therefore \boxed{z = 2}$$

$$\text{from (1), } x + 3(1) + 2(2) = 6$$

$$\therefore x = 6 - 7$$

$$\therefore \boxed{x = -1}$$

$$\therefore x = -1, y = 1, z = 2$$

Sign of Teacher :